<?xml version="1.0"?>


<!DOCTYPE rdf:RDF [
    <!ENTITY void "http://rdfs.org/ns/void#" >
    <!ENTITY dcterms "http://purl.org/dc/terms/" >
    <!ENTITY vann "http://purl.org/vocab/vann/" >
    <!ENTITY owl "http://www.w3.org/2002/07/owl#" >
    <!ENTITY xsd "http://www.w3.org/2001/XMLSchema#" >
    <!ENTITY ontolex "http://www.w3.org/ns/lemon/ontolex#" >
    <!ENTITY rdfs "http://www.w3.org/2000/01/rdf-schema#" >
    <!ENTITY rdf "http://www.w3.org/1999/02/22-rdf-syntax-ns#" >
]>


<rdf:RDF xmlns="http://www.w3.org/ns/lemon/lime#"
     xml:base="http://www.w3.org/ns/lemon/lime"
     xmlns:rdfs="http://www.w3.org/2000/01/rdf-schema#"
     xmlns:ontolex="http://www.w3.org/ns/lemon/ontolex#"
     xmlns:owl="http://www.w3.org/2002/07/owl#"
     xmlns:xsd="http://www.w3.org/2001/XMLSchema#"
     xmlns:rdf="http://www.w3.org/1999/02/22-rdf-syntax-ns#"
     xmlns:void="http://rdfs.org/ns/void#"
     xmlns:vann="http://purl.org/vocab/vann/"
     xmlns:dcterms="http://purl.org/dc/terms/">
    <owl:Ontology rdf:about="http://www.w3.org/ns/lemon/lime">
        <rdfs:label xml:lang="en">LIngusitic MEtadata (LIME)</rdfs:label>
        <vann:preferredNamespaceUri rdf:datatype="&xsd;string">http://www.w3.org/ns/lemon/lime#</vann:preferredNamespaceUri>
        <vann:preferredNamespacePrefix rdf:datatype="&xsd;string">lime</vann:preferredNamespacePrefix>
        <dcterms:description xml:lang="en">LIME (LInguistic MEtadata) is a vocabulary for expressing linguistic metadata about linguistic resources and linguistically grounded datasets.</dcterms:description>
        <dcterms:title xml:lang="en">Vocabulary of Linguistic Metadata</dcterms:title>
        <owl:imports rdf:resource="http://rdfs.org/ns/void"/>
        <owl:imports rdf:resource="http://www.w3.org/ns/lemon/ontolex"/>
    </owl:Ontology>
    


    <!-- 
    ///////////////////////////////////////////////////////////////////////////////////////
    //
    // Object Properties
    //
    ///////////////////////////////////////////////////////////////////////////////////////
     -->

    


    <!-- http://www.w3.org/ns/lemon/lime#conceptualDataset -->

    <owl:ObjectProperty rdf:about="http://www.w3.org/ns/lemon/lime#conceptualDataset">
        <rdfs:label xml:lang="en">conceptual dataset</rdfs:label>
        <rdfs:comment xml:lang="en">The concept set referred to by a lexical linkset</rdfs:comment>
        <rdfs:isDefinedBy>http://www.w3.org/ns/lemon/lime</rdfs:isDefinedBy>
        <rdfs:domain rdf:resource="http://www.w3.org/ns/lemon/lime#LexicalLinkset"/>
        <rdfs:range rdf:resource="&ontolex;ConceptSet"/>
    </owl:ObjectProperty>
    


    <!-- http://www.w3.org/ns/lemon/lime#lexicalizationModel -->

    <owl:ObjectProperty rdf:about="http://www.w3.org/ns/lemon/lime#lexicalizationModel">
        <rdfs:label xml:lang="en">lexicalization model</rdfs:label>
        <rdfs:isDefinedBy>http://www.w3.org/ns/lemon/lime</rdfs:isDefinedBy>
    </owl:ObjectProperty>
    


    <!-- http://www.w3.org/ns/lemon/lime#lexiconDataset -->

    <owl:ObjectProperty rdf:about="http://www.w3.org/ns/lemon/lime#lexiconDataset">
        <rdf:type rdf:resource="&owl;FunctionalProperty"/>
        <rdfs:label xml:lang="en">lexicon dataset</rdfs:label>
        <rdfs:comment xml:lang="en">The &apos;lexicon dataset&apos; property indicates the lexicon that contains the entries refered to in the lexicalization set or conceptualization. </rdfs:comment>
        <rdfs:isDefinedBy rdf:resource="http://www.w3.org/ns/lemon/lime"/>
        <rdfs:domain rdf:resource="http://www.w3.org/ns/lemon/lime#LexicalizationSet"/>
        <rdfs:range rdf:resource="&ontolex;Lexicon"/>
    </owl:ObjectProperty>
    


    <!-- http://www.w3.org/ns/lemon/lime#linguisticModel -->

    <owl:ObjectProperty rdf:about="http://www.w3.org/ns/lemon/lime#linguisticModel">
        <rdfs:label xml:lang="en">linguistic model</rdfs:label>
        <rdfs:comment xml:lang="en">The &apos;linguistic model&apos; property indicates the catalog of linguistic categories used in a lexicon to define linguistic properties of lexical entries. </rdfs:comment>
        <rdfs:isDefinedBy>http://www.w3.org/ns/lemon/lime</rdfs:isDefinedBy>
        <rdfs:domain rdf:resource="&ontolex;Lexicon"/>
    </owl:ObjectProperty>
    


    <!-- http://www.w3.org/ns/lemon/lime#partition -->

    <owl:ObjectProperty rdf:about="http://www.w3.org/ns/lemon/lime#partition">
        <rdfs:label xml:lang="en">partition</rdfs:label>
        <rdfs:comment xml:lang="en">Statistics about the lexicalization set or lexical link set for resources of a given type.</rdfs:comment>
        <rdfs:isDefinedBy rdf:resource="http://www.w3.org/ns/lemon/lime"/>
    </owl:ObjectProperty>
    


    <!-- http://www.w3.org/ns/lemon/lime#referenceDataset -->

    <owl:ObjectProperty rdf:about="http://www.w3.org/ns/lemon/lime#referenceDataset">
        <rdf:type rdf:resource="&owl;FunctionalProperty"/>
        <rdfs:label xml:lang="en">reference dataset</rdfs:label>
        <rdfs:comment xml:lang="en">The &apos;reference dataset&apos; property indicates the dataset that contains the ontology or vocabulary elements referenced by a given lexicon and thus providing the gronuding vocabulary for the meaning of the lexical entries in the lexicon.</rdfs:comment>
        <rdfs:range rdf:resource="&void;Dataset"/>
        <rdfs:isDefinedBy rdf:resource="http://www.w3.org/ns/lemon/lime"/>
        <rdfs:domain>
            <owl:Class>
                <owl:unionOf rdf:parseType="Collection">
                    <rdf:Description rdf:about="http://www.w3.org/ns/lemon/lime#LexicalLinkset"/>
                    <rdf:Description rdf:about="http://www.w3.org/ns/lemon/lime#LexicalizationSet"/>
                </owl:unionOf>
            </owl:Class>
        </rdfs:domain>
    </owl:ObjectProperty>
    


    <!-- http://www.w3.org/ns/lemon/lime#resourceType -->

    <owl:ObjectProperty rdf:about="http://www.w3.org/ns/lemon/lime#resourceType">
        <rdf:type rdf:resource="&owl;FunctionalProperty"/>
        <rdfs:label xml:lang="en">resource type</rdfs:label>
        <rdfs:comment xml:lang="en">The type of resources for a given partition</rdfs:comment>
        <rdfs:isDefinedBy>http://www.w3.org/ns/lemon/lime</rdfs:isDefinedBy>
        <rdfs:range rdf:resource="&rdfs;Class"/>
        <rdfs:domain>
            <owl:Class>
                <owl:unionOf rdf:parseType="Collection">
                    <rdf:Description rdf:about="http://www.w3.org/ns/lemon/lime#LexicalLinkset"/>
                    <rdf:Description rdf:about="http://www.w3.org/ns/lemon/lime#LexicalizationSet"/>
                </owl:unionOf>
            </owl:Class>
        </rdfs:domain>
    </owl:ObjectProperty>
    


    <!-- 
    ///////////////////////////////////////////////////////////////////////////////////////
    //
    // Data properties
    //
    ///////////////////////////////////////////////////////////////////////////////////////
     -->

    


    <!-- http://www.w3.org/ns/lemon/lime#avgNumOfLexicalizations -->

    <owl:DatatypeProperty rdf:about="http://www.w3.org/ns/lemon/lime#avgNumOfLexicalizations">
        <rdfs:label xml:lang="en">average number of lexicalizations</rdfs:label>
        <rdfs:isDefinedBy>http://www.w3.org/ns/lemon/lime</rdfs:isDefinedBy>
        <rdfs:comment xml:lang="en">The average number of lexicalizations for each of reference.</rdfs:comment>
        <rdfs:range rdf:resource="&xsd;decimal"/>
        <rdfs:domain rdf:resource="http://www.w3.org/ns/lemon/lime#LexicalizationSet"/>
    </owl:DatatypeProperty>
    


    <!-- http://www.w3.org/ns/lemon/lime#avgNumOfLinks -->

    <owl:DatatypeProperty rdf:about="http://www.w3.org/ns/lemon/lime#avgNumOfLinks">
        <rdfs:label xml:lang="en">average number of links</rdfs:label>
        <rdfs:comment xml:lang="en">The average number of links for each entity in the reference dataset</rdfs:comment>
        <rdfs:isDefinedBy>http://www.w3.org/ns/lemon/lime</rdfs:isDefinedBy>
        <rdfs:range rdf:resource="&xsd;decimal"/>
        <rdfs:domain rdf:resource="http://www.w3.org/ns/lemon/lime#LexicalLinkset"/>
    </owl:DatatypeProperty>
    


    <!-- http://www.w3.org/ns/lemon/lime#concepts -->

    <owl:DatatypeProperty rdf:about="http://www.w3.org/ns/lemon/lime#concepts">
        <rdfs:label xml:lang="en">concepts</rdfs:label>
        <rdfs:comment xml:lang="en">The number of lexical concepts in a concept set or lexical linkset</rdfs:comment>
        <rdfs:isDefinedBy xml:lang="en">http://www.w3.org/ns/lemon/lime</rdfs:isDefinedBy>
        <rdfs:range rdf:resource="&xsd;integer"/>
        <rdfs:domain>
            <owl:Class>
                <owl:unionOf rdf:parseType="Collection">
                    <rdf:Description rdf:about="http://www.w3.org/ns/lemon/lime#LexicalLinkset"/>
                    <rdf:Description rdf:about="&ontolex;ConceptSet"/>
                </owl:unionOf>
            </owl:Class>
        </rdfs:domain>
    </owl:DatatypeProperty>
    


    <!-- http://www.w3.org/ns/lemon/lime#lexicalEntries -->

    <owl:DatatypeProperty rdf:about="http://www.w3.org/ns/lemon/lime#lexicalEntries">
        <rdfs:label xml:lang="en">lexical entries</rdfs:label>
        <rdfs:comment xml:lang="en">The &apos;lexical entries&apos; property indicates the number of distinct lexical entries contained in a lexicon or lexicalization set. </rdfs:comment>
        <rdfs:range rdf:resource="&xsd;integer"/>
        <rdfs:isDefinedBy rdf:resource="http://www.w3.org/ns/lemon/lime"/>
        <rdfs:domain>
            <owl:Class>
                <owl:unionOf rdf:parseType="Collection">
                    <rdf:Description rdf:about="http://www.w3.org/ns/lemon/lime#LexicalizationSet"/>
                    <rdf:Description rdf:about="&ontolex;Lexicon"/>
                </owl:unionOf>
            </owl:Class>
        </rdfs:domain>
    </owl:DatatypeProperty>
    


    <!-- http://www.w3.org/ns/lemon/lime#lexicalizations -->

    <owl:DatatypeProperty rdf:about="http://www.w3.org/ns/lemon/lime#lexicalizations">
        <rdfs:label xml:lang="en">lexicalizations</rdfs:label>
        <rdfs:comment xml:lang="en">Number of distinct lexicalizations.</rdfs:comment>
        <rdfs:range rdf:resource="&xsd;integer"/>
        <rdfs:isDefinedBy rdf:resource="http://www.w3.org/ns/lemon/lime"/>
        <rdfs:domain rdf:resource="http://www.w3.org/ns/lemon/lime#LexicalizationSet"/>
    </owl:DatatypeProperty>
    


    <!-- http://www.w3.org/ns/lemon/lime#links -->

    <owl:DatatypeProperty rdf:about="http://www.w3.org/ns/lemon/lime#links">
        <rdfs:label xml:lang="en">links</rdfs:label>
        <rdfs:comment xml:lang="en">The number of links between concepts in the concepts set and entities in the reference dataset</rdfs:comment>
        <rdfs:isDefinedBy>http://www.w3.org/ns/lemon/lime</rdfs:isDefinedBy>
        <rdfs:range rdf:resource="&xsd;integer"/>
        <rdfs:domain rdf:resource="http://www.w3.org/ns/lemon/lime#LexicalLinkset"/>
    </owl:DatatypeProperty>
    


    <!-- http://www.w3.org/ns/lemon/lime#percentage -->

    <owl:DatatypeProperty rdf:about="http://www.w3.org/ns/lemon/lime#percentage">
        <rdfs:label xml:lang="en">percentage</rdfs:label>
        <rdfs:comment xml:lang="en">Percentage of entities in the reference dataset which have at least one lexicalization</rdfs:comment>
        <rdfs:isDefinedBy>http://www.w3.org/ns/lemon/lime</rdfs:isDefinedBy>
        <rdfs:range rdf:resource="&xsd;decimal"/>
        <rdfs:domain>
            <owl:Class>
                <owl:unionOf rdf:parseType="Collection">
                    <rdf:Description rdf:about="http://www.w3.org/ns/lemon/lime#LexicalLinkset"/>
                    <rdf:Description rdf:about="http://www.w3.org/ns/lemon/lime#LexicalizationSet"/>
                </owl:unionOf>
            </owl:Class>
        </rdfs:domain>
    </owl:DatatypeProperty>
    


    <!-- http://www.w3.org/ns/lemon/lime#references -->

    <owl:DatatypeProperty rdf:about="http://www.w3.org/ns/lemon/lime#references">
        <rdfs:label xml:lang="en">references</rdfs:label>
        <rdfs:comment xml:lang="en">The &apos;references&apos; property indicates the number of distinct references in the ontology vocabulary lexicalized by at least one lexical entry.</rdfs:comment>
        <rdfs:range rdf:resource="&xsd;integer"/>
        <rdfs:isDefinedBy rdf:resource="http://www.w3.org/ns/lemon/lime"/>
        <rdfs:domain rdf:resource="http://www.w3.org/ns/lemon/lime#LexicalizationSet"/>
    </owl:DatatypeProperty>
    


    <!-- 
    ///////////////////////////////////////////////////////////////////////////////////////
    //
    // Classes
    //
    ///////////////////////////////////////////////////////////////////////////////////////
     -->

    


    <!-- http://rdfs.org/ns/void#Linkset -->

    <owl:Class rdf:about="&void;Linkset"/>
    


    <!-- http://www.w3.org/2000/01/rdf-schema#Class -->

    <owl:Class rdf:about="&rdfs;Class"/>
    


    <!-- http://www.w3.org/ns/lemon/lime#LexicalLinkset -->

    <owl:Class rdf:about="http://www.w3.org/ns/lemon/lime#LexicalLinkset">
        <rdfs:label xml:lang="en">Lexical linkset</rdfs:label>
        <rdfs:subClassOf rdf:resource="&void;Linkset"/>
        <rdfs:subClassOf>
            <owl:Restriction>
                <owl:onProperty rdf:resource="http://www.w3.org/ns/lemon/lime#referenceDataset"/>
                <owl:onClass rdf:resource="&void;Dataset"/>
                <owl:qualifiedCardinality rdf:datatype="&xsd;nonNegativeInteger">1</owl:qualifiedCardinality>
            </owl:Restriction>
        </rdfs:subClassOf>
        <rdfs:subClassOf>
            <owl:Restriction>
                <owl:onProperty rdf:resource="http://www.w3.org/ns/lemon/lime#conceptualDataset"/>
                <owl:onClass rdf:resource="&ontolex;ConceptSet"/>
                <owl:qualifiedCardinality rdf:datatype="&xsd;nonNegativeInteger">1</owl:qualifiedCardinality>
            </owl:Restriction>
        </rdfs:subClassOf>
        <rdfs:subClassOf>
            <owl:Restriction>
                <owl:onProperty rdf:resource="http://www.w3.org/ns/lemon/lime#partition"/>
                <owl:allValuesFrom rdf:resource="http://www.w3.org/ns/lemon/lime#LexicalLinkset"/>
            </owl:Restriction>
        </rdfs:subClassOf>
        <rdfs:comment xml:lang="en">A  lexical linkset provides a collection of links between an RDF dataset and a conceptualized linguistic resource (e.g., WordNet).</rdfs:comment>
        <rdfs:isDefinedBy rdf:resource="http://www.w3.org/ns/lemon/lime"/>
    </owl:Class>
    


    <!-- http://www.w3.org/ns/lemon/lime#LexicalizationSet -->

    <owl:Class rdf:about="http://www.w3.org/ns/lemon/lime#LexicalizationSet">
        <rdfs:subClassOf rdf:resource="&void;Dataset"/>
        <rdfs:subClassOf>
            <owl:Restriction>
                <owl:onProperty rdf:resource="http://www.w3.org/ns/lemon/lime#lexiconDataset"/>
                <owl:onClass rdf:resource="&ontolex;Lexicon"/>
                <owl:qualifiedCardinality rdf:datatype="&xsd;nonNegativeInteger">1</owl:qualifiedCardinality>
            </owl:Restriction>
        </rdfs:subClassOf>
        <rdfs:subClassOf>
            <owl:Restriction>
                <owl:onProperty rdf:resource="http://www.w3.org/ns/lemon/lime#partition"/>
                <owl:allValuesFrom rdf:resource="http://www.w3.org/ns/lemon/lime#LexicalizationSet"/>
            </owl:Restriction>
        </rdfs:subClassOf>
        <rdfs:subClassOf>
            <owl:Restriction>
                <owl:onProperty rdf:resource="http://www.w3.org/ns/lemon/lime#referenceDataset"/>
                <owl:onClass rdf:resource="&void;Dataset"/>
                <owl:qualifiedCardinality rdf:datatype="&xsd;nonNegativeInteger">1</owl:qualifiedCardinality>
            </owl:Restriction>
        </rdfs:subClassOf>
        <rdfs:comment xml:lang="en">A &apos;lexicalization set&apos; is a dataset that comprises a collection of lexicalizations, that is pairs of lexical entry and associated reference in the ontology/vocabulary/dataset.</rdfs:comment>
        <rdfs:isDefinedBy rdf:resource="http://www.w3.org/ns/lemon/lime"/>
    </owl:Class>
</rdf:RDF>



<!-- Generated by the OWL API (version 3.4.2) http://owlapi.sourceforge.net -->

