<?xml version="1.0"?>


<!DOCTYPE rdf:RDF [
    <!ENTITY owl "http://www.w3.org/2002/07/owl#" >
    <!ENTITY xsd "http://www.w3.org/2001/XMLSchema#" >
    <!ENTITY ontolex "http://www.w3.org/ns/lemon/ontolex#" >
    <!ENTITY owl2xml "http://www.w3.org/2006/12/owl2-xml#" >
    <!ENTITY rdfs "http://www.w3.org/2000/01/rdf-schema#" >
    <!ENTITY rdf "http://www.w3.org/1999/02/22-rdf-syntax-ns#" >
    <!ENTITY semiotics "http://www.ontologydesignpatterns.org/cp/owl/semiotics.owl#" >
]>


<rdf:RDF xmlns="http://www.w3.org/ns/lemon/ontolex#"
     xml:base="http://www.w3.org/ns/lemon/ontolex"
     xmlns:semiotics="http://www.ontologydesignpatterns.org/cp/owl/semiotics.owl#"
     xmlns:rdfs="http://www.w3.org/2000/01/rdf-schema#"
     xmlns:owl2xml="http://www.w3.org/2006/12/owl2-xml#"
     xmlns:ontolex="http://www.w3.org/ns/lemon/ontolex#"
     xmlns:owl="http://www.w3.org/2002/07/owl#"
     xmlns:xsd="http://www.w3.org/2001/XMLSchema#"
     xmlns:rdf="http://www.w3.org/1999/02/22-rdf-syntax-ns#">
    <owl:Ontology rdf:about="http://www.w3.org/ns/lemon/ontolex"/>
    


    <!-- 
    ///////////////////////////////////////////////////////////////////////////////////////
    //
    // Datatypes
    //
    ///////////////////////////////////////////////////////////////////////////////////////
     -->

    


    <!-- http://www.w3.org/1999/02/22-rdf-syntax-ns#langString -->

    <rdfs:Datatype rdf:about="&rdf;langString"/>
    


    <!-- 
    ///////////////////////////////////////////////////////////////////////////////////////
    //
    // Object Properties
    //
    ///////////////////////////////////////////////////////////////////////////////////////
     -->

    


    <!-- http://www.ontologydesignpatterns.org/cp/owl/semiotics.owl#denotes -->

    <owl:ObjectProperty rdf:about="&semiotics;denotes"/>
    


    <!-- http://www.w3.org/2002/07/owl#topObjectProperty -->

    <owl:ObjectProperty rdf:about="&owl;topObjectProperty"/>
    


    <!-- http://www.w3.org/2004/02/skos/core#inScheme -->

    <owl:ObjectProperty rdf:about="http://www.w3.org/2004/02/skos/core#inScheme"/>
    


    <!-- http://www.w3.org/ns/lemon/ontolex#canonicalForm -->

    <owl:ObjectProperty rdf:about="&ontolex;canonicalForm">
        <rdf:type rdf:resource="&owl;FunctionalProperty"/>
        <rdfs:comment xml:lang="en">The object property canonical form relates a lexical entry to its canoncical or dictionary form. This usually indicates the &quot;lemma&quot; form of a lexical entry. </rdfs:comment>
        <rdfs:range rdf:resource="&ontolex;Form"/>
        <rdfs:domain rdf:resource="&ontolex;LexicalEntry"/>
        <rdfs:subPropertyOf rdf:resource="&ontolex;lexicalForm"/>
    </owl:ObjectProperty>
    


    <!-- http://www.w3.org/ns/lemon/ontolex#concept -->

    <owl:ObjectProperty rdf:about="&ontolex;concept">
        <rdfs:comment xml:lang="en">The object property concept relates an ontological entity to a Lexical Concept that represents the corresponding meaning. </rdfs:comment>
        <rdfs:range rdf:resource="&ontolex;LexicalConcept"/>
    </owl:ObjectProperty>
    


    <!-- http://www.w3.org/ns/lemon/ontolex#definition -->

    <owl:ObjectProperty rdf:about="&ontolex;definition">
        <rdfs:comment xml:lang="en">The object property definition relates a LexicalSense to one of its defintions; multiple definitions are allowed. </rdfs:comment>
        <rdfs:domain>
            <owl:Class>
                <owl:unionOf rdf:parseType="Collection">
                    <rdf:Description rdf:about="&ontolex;LexicalConcept"/>
                    <rdf:Description rdf:about="&ontolex;LexicalSense"/>
                </owl:unionOf>
            </owl:Class>
        </rdfs:domain>
    </owl:ObjectProperty>
    


    <!-- http://www.w3.org/ns/lemon/ontolex#denotes -->

    <owl:ObjectProperty rdf:about="&ontolex;denotes">
        <rdfs:comment xml:lang="en">The object property denotes relates a lexical entry to a predicate in a given ontology that represents its meaning and has some denotational or model-theoretic semantics. </rdfs:comment>
        <rdfs:subPropertyOf rdf:resource="&semiotics;denotes"/>
        <rdfs:domain rdf:resource="&ontolex;LexicalEntry"/>
        <owl:propertyChainAxiom rdf:parseType="Collection">
            <rdf:Description rdf:about="&ontolex;sense"/>
            <rdf:Description rdf:about="&ontolex;reference"/>
        </owl:propertyChainAxiom>
    </owl:ObjectProperty>
    


    <!-- http://www.w3.org/ns/lemon/ontolex#entry -->

    <owl:ObjectProperty rdf:about="&ontolex;entry">
        <rdfs:comment xml:lang="en">The object property entry relates a lexicon to one of the lexical entries contained in it. </rdfs:comment>
        <rdfs:range rdf:resource="&ontolex;LexicalEntry"/>
        <rdfs:domain rdf:resource="&ontolex;Lexicon"/>
    </owl:ObjectProperty>
    


    <!-- http://www.w3.org/ns/lemon/ontolex#evokes -->

    <owl:ObjectProperty rdf:about="&ontolex;evokes">
        <rdfs:comment xml:lang="en">The object property evokes relates a lexical entry to one of the lexical concepts it evokes, i.e. the mental concept that speakers of a language might associate when hearing the lexical entry.</rdfs:comment>
        <rdfs:range rdf:resource="&ontolex;LexicalConcept"/>
        <rdfs:domain rdf:resource="&ontolex;LexicalEntry"/>
        <owl:propertyChainAxiom rdf:parseType="Collection">
            <rdf:Description rdf:about="&ontolex;sense"/>
            <rdf:Description rdf:about="&ontolex;isLexicalizedSenseOf"/>
        </owl:propertyChainAxiom>
    </owl:ObjectProperty>
    


    <!-- http://www.w3.org/ns/lemon/ontolex#isConceptOf -->

    <owl:ObjectProperty rdf:about="&ontolex;isConceptOf">
        <rdfs:comment xml:lang="en">This property formalizes the meaning of a Lexical Concept by linking it to a particular ontological meaning.</rdfs:comment>
        <rdfs:domain rdf:resource="&ontolex;LexicalConcept"/>
    </owl:ObjectProperty>
    


    <!-- http://www.w3.org/ns/lemon/ontolex#isDenotedBy -->

    <owl:ObjectProperty rdf:about="&ontolex;isDenotedBy">
        <rdfs:comment xml:lang="en">The object property isDenotedBy is the inverse of the object property denotes.</rdfs:comment>
        <rdfs:range rdf:resource="&ontolex;LexicalEntry"/>
        <owl:inverseOf rdf:resource="&ontolex;denotes"/>
    </owl:ObjectProperty>
    


    <!-- http://www.w3.org/ns/lemon/ontolex#isEvokedBy -->

    <owl:ObjectProperty rdf:about="&ontolex;isEvokedBy">
        <rdfs:comment xml:lang="en">The inverse relation to evokes.</rdfs:comment>
        <rdfs:domain rdf:resource="&ontolex;LexicalConcept"/>
        <rdfs:range rdf:resource="&ontolex;LexicalEntry"/>
        <owl:inverseOf rdf:resource="&ontolex;evokes"/>
    </owl:ObjectProperty>
    


    <!-- http://www.w3.org/ns/lemon/ontolex#isLexicalizedSenseOf -->

    <owl:ObjectProperty rdf:about="&ontolex;isLexicalizedSenseOf">
        <rdfs:comment xml:lang="en">The object property isLexicalizedSenseOf is the inverse property of lexicalized sense.</rdfs:comment>
        <rdfs:domain rdf:resource="&ontolex;LexicalConcept"/>
        <rdfs:range rdf:resource="&ontolex;LexicalSense"/>
        <owl:inverseOf rdf:resource="&ontolex;lexicalizedSense"/>
    </owl:ObjectProperty>
    


    <!-- http://www.w3.org/ns/lemon/ontolex#isReferenceOf -->

    <owl:ObjectProperty rdf:about="&ontolex;isReferenceOf">
        <rdf:type rdf:resource="&owl;InverseFunctionalProperty"/>
        <rdfs:comment xml:lang="en">The object property isReferenceOf is the inverse property of reference.</rdfs:comment>
        <rdfs:range rdf:resource="&ontolex;LexicalSense"/>
        <owl:inverseOf rdf:resource="&ontolex;reference"/>
    </owl:ObjectProperty>
    


    <!-- http://www.w3.org/ns/lemon/ontolex#isSenseOf -->

    <owl:ObjectProperty rdf:about="&ontolex;isSenseOf">
        <rdf:type rdf:resource="&owl;FunctionalProperty"/>
        <rdfs:comment xml:lang="en">The property isSenseOf is the inverse property of sense.</rdfs:comment>
        <rdfs:range rdf:resource="&ontolex;LexicalEntry"/>
        <rdfs:domain rdf:resource="&ontolex;LexicalSense"/>
    </owl:ObjectProperty>
    


    <!-- http://www.w3.org/ns/lemon/ontolex#lexicalForm -->

    <owl:ObjectProperty rdf:about="&ontolex;lexicalForm">
        <rdfs:comment xml:lang="en">The object property lexical form relates a lexical entry to one grammatical form variant of the lexical entry. </rdfs:comment>
        <rdfs:range rdf:resource="&ontolex;Form"/>
        <rdfs:domain rdf:resource="&ontolex;LexicalEntry"/>
    </owl:ObjectProperty>
    


    <!-- http://www.w3.org/ns/lemon/ontolex#lexicalizedSense -->

    <owl:ObjectProperty rdf:about="&ontolex;lexicalizedSense">
        <rdfs:comment xml:lang="en">The object property lexicalized sense relates a lexical concept and a corresponding lexical sense that lexicalizes the lexical concept. </rdfs:comment>
        <rdfs:domain rdf:resource="&ontolex;LexicalConcept"/>
        <rdfs:range rdf:resource="&ontolex;LexicalSense"/>
    </owl:ObjectProperty>
    


    <!-- http://www.w3.org/ns/lemon/ontolex#morphologicalPattern -->

    <owl:ObjectProperty rdf:about="&ontolex;morphologicalPattern">
        <rdfs:comment xml:lang="en">The object property morphological pattern indicates the morphological class of a word. </rdfs:comment>
        <rdfs:domain rdf:resource="&ontolex;LexicalEntry"/>
    </owl:ObjectProperty>
    


    <!-- http://www.w3.org/ns/lemon/ontolex#otherForm -->

    <owl:ObjectProperty rdf:about="&ontolex;otherForm">
        <rdfs:comment xml:lang="en">The object property other form relates a lexical entry to a non-preferred (&quot;non-dictionary&quot;) representation of it. This should be a variant that is either a morphological variant, an abbreviation, short form or acronym.</rdfs:comment>
        <rdfs:range rdf:resource="&ontolex;Form"/>
        <rdfs:domain rdf:resource="&ontolex;LexicalEntry"/>
        <rdfs:subPropertyOf rdf:resource="&ontolex;lexicalForm"/>
    </owl:ObjectProperty>
    


    <!-- http://www.w3.org/ns/lemon/ontolex#reference -->

    <owl:ObjectProperty rdf:about="&ontolex;reference">
        <rdf:type rdf:resource="&owl;FunctionalProperty"/>
        <rdfs:comment xml:lang="en">The object property reference relates a lexical sense to an ontological predicate that represents the denotation of the corresponding lexical entry. </rdfs:comment>
        <rdfs:domain rdf:resource="&ontolex;LexicalSense"/>
    </owl:ObjectProperty>
    


    <!-- http://www.w3.org/ns/lemon/ontolex#sense -->

    <owl:ObjectProperty rdf:about="&ontolex;sense">
        <rdf:type rdf:resource="&owl;InverseFunctionalProperty"/>
        <rdfs:comment xml:lang="en">The object property sense relates a lexical entry to one of its lexical senses. </rdfs:comment>
        <rdfs:domain rdf:resource="&ontolex;LexicalEntry"/>
        <rdfs:range rdf:resource="&ontolex;LexicalSense"/>
        <owl:inverseOf rdf:resource="&ontolex;isSenseOf"/>
    </owl:ObjectProperty>
    


    <!-- 
    ///////////////////////////////////////////////////////////////////////////////////////
    //
    // Data properties
    //
    ///////////////////////////////////////////////////////////////////////////////////////
     -->

    


    <!-- http://www.w3.org/2002/07/owl#topDataProperty -->

    <owl:DatatypeProperty rdf:about="&owl;topDataProperty"/>
    


    <!-- http://www.w3.org/ns/lemon/ontolex#language -->

    <owl:DatatypeProperty rdf:about="&ontolex;language">
        <rdfs:comment xml:lang="en">The datatype property language indicates the language of a lexicon or an individual lexical entry. </rdfs:comment>
        <rdfs:range rdf:resource="&rdfs;Literal"/>
        <rdfs:subPropertyOf rdf:resource="&owl;topDataProperty"/>
        <rdfs:domain>
            <owl:Class>
                <owl:unionOf rdf:parseType="Collection">
                    <rdf:Description rdf:about="http://www.w3.org/ns/lemon/lime#LexicalizationSet"/>
                    <rdf:Description rdf:about="&ontolex;ConceptSet"/>
                    <rdf:Description rdf:about="&ontolex;LexicalEntry"/>
                    <rdf:Description rdf:about="&ontolex;Lexicon"/>
                </owl:unionOf>
            </owl:Class>
        </rdfs:domain>
    </owl:DatatypeProperty>
    <owl:Axiom>
        <rdfs:comment></rdfs:comment>
        <owl:annotatedTarget xml:lang="en">The datatype property language indicates the language of a lexicon or an individual lexical entry. </owl:annotatedTarget>
        <owl:annotatedProperty rdf:resource="&rdfs;comment"/>
        <owl:annotatedSource rdf:resource="&ontolex;language"/>
    </owl:Axiom>
    


    <!-- http://www.w3.org/ns/lemon/ontolex#phoneticRep -->

    <owl:DatatypeProperty rdf:about="&ontolex;phoneticRep">
        <rdfs:comment xml:lang="en">The datatype property phonetic representation indicates one phonetic representation of the pronunciation of the form using a scheme such as the International Phonetic Alphabet (IPA). </rdfs:comment>
        <rdfs:range rdf:resource="&rdf;langString"/>
        <rdfs:domain rdf:resource="&ontolex;Form"/>
        <rdfs:subPropertyOf rdf:resource="&ontolex;representation"/>
    </owl:DatatypeProperty>
    


    <!-- http://www.w3.org/ns/lemon/ontolex#representation -->

    <owl:DatatypeProperty rdf:about="&ontolex;representation">
        <rdfs:comment xml:lang="en">The datatype property representation indicates a string by which the form is represented according to some scheme. </rdfs:comment>
        <rdfs:range rdf:resource="&rdf;langString"/>
        <rdfs:domain rdf:resource="&ontolex;Form"/>
    </owl:DatatypeProperty>
    


    <!-- http://www.w3.org/ns/lemon/ontolex#writtenRep -->

    <owl:DatatypeProperty rdf:about="&ontolex;writtenRep">
        <rdfs:comment xml:lang="en">The datatype property written representation indicates the written representation of a form. </rdfs:comment>
        <rdfs:range rdf:resource="&rdf;langString"/>
        <rdfs:domain rdf:resource="&ontolex;Form"/>
        <rdfs:subPropertyOf rdf:resource="&ontolex;representation"/>
    </owl:DatatypeProperty>
    


    <!-- 
    ///////////////////////////////////////////////////////////////////////////////////////
    //
    // Classes
    //
    ///////////////////////////////////////////////////////////////////////////////////////
     -->

    


    <!-- http://rdfs.org/ns/void#Dataset -->

    <owl:Class rdf:about="http://rdfs.org/ns/void#Dataset"/>
    


    <!-- http://www.ontologydesignpatterns.org/cp/owl/semiotics.owl#Expression -->

    <owl:Class rdf:about="&semiotics;Expression"/>
    


    <!-- http://www.ontologydesignpatterns.org/cp/owl/semiotics.owl#Meaning -->

    <owl:Class rdf:about="&semiotics;Meaning"/>
    


    <!-- http://www.w3.org/2004/02/skos/core#Concept -->

    <owl:Class rdf:about="http://www.w3.org/2004/02/skos/core#Concept"/>
    


    <!-- http://www.w3.org/2004/02/skos/core#ConceptScheme -->

    <owl:Class rdf:about="http://www.w3.org/2004/02/skos/core#ConceptScheme"/>
    


    <!-- http://www.w3.org/ns/lemon/lime#LexicalizationSet -->

    <owl:Class rdf:about="http://www.w3.org/ns/lemon/lime#LexicalizationSet"/>
    


    <!-- http://www.w3.org/ns/lemon/ontolex#Affix -->

    <owl:Class rdf:about="&ontolex;Affix">
        <rdfs:subClassOf rdf:resource="&ontolex;LexicalEntry"/>
        <rdfs:comment xml:lang="en">The class affix represents a lexical entry which is realized by joining it as a prefix or similar to another word.
</rdfs:comment>
    </owl:Class>
    


    <!-- http://www.w3.org/ns/lemon/ontolex#ConceptSet -->

    <owl:Class rdf:about="&ontolex;ConceptSet">
        <owl:equivalentClass>
            <owl:Restriction>
                <owl:onProperty rdf:resource="http://www.w3.org/2004/02/skos/core#inScheme"/>
                <owl:onClass rdf:resource="&ontolex;LexicalConcept"/>
                <owl:minQualifiedCardinality rdf:datatype="&xsd;nonNegativeInteger">1</owl:minQualifiedCardinality>
            </owl:Restriction>
        </owl:equivalentClass>
        <rdfs:subClassOf rdf:resource="http://www.w3.org/2004/02/skos/core#ConceptScheme"/>
        <rdfs:comment xml:lang="en">The class concept set represents a collection of lexical concepts.</rdfs:comment>
    </owl:Class>
    


    <!-- http://www.w3.org/ns/lemon/ontolex#Form -->

    <owl:Class rdf:about="&ontolex;Form">
        <rdfs:subClassOf rdf:resource="&owl;Thing"/>
        <rdfs:subClassOf>
            <owl:Restriction>
                <owl:onProperty rdf:resource="&ontolex;writtenRep"/>
                <owl:minCardinality rdf:datatype="&xsd;nonNegativeInteger">1</owl:minCardinality>
            </owl:Restriction>
        </rdfs:subClassOf>
        <rdfs:comment xml:lang="en">The class form represents one grammatical realization of a lexical entry. </rdfs:comment>
    </owl:Class>
    


    <!-- http://www.w3.org/ns/lemon/ontolex#LexicalConcept -->

    <owl:Class rdf:about="&ontolex;LexicalConcept">
        <rdfs:subClassOf rdf:resource="http://www.w3.org/2004/02/skos/core#Concept"/>
        <rdfs:comment xml:lang="en">The class lexical concept represents a mental abstraction, concept or unit of thought that can be lexicalized by a given collection of senses. </rdfs:comment>
    </owl:Class>
    


    <!-- http://www.w3.org/ns/lemon/ontolex#LexicalEntry -->

    <owl:Class rdf:about="&ontolex;LexicalEntry">
        <rdfs:subClassOf rdf:resource="&semiotics;Expression"/>
        <rdfs:subClassOf rdf:resource="&owl;Thing"/>
        <rdfs:subClassOf>
            <owl:Restriction>
                <owl:onProperty rdf:resource="&ontolex;lexicalForm"/>
                <owl:onClass rdf:resource="&ontolex;Form"/>
                <owl:minQualifiedCardinality rdf:datatype="&xsd;nonNegativeInteger">1</owl:minQualifiedCardinality>
            </owl:Restriction>
        </rdfs:subClassOf>
        <rdfs:subClassOf>
            <owl:Restriction>
                <owl:onProperty rdf:resource="&ontolex;canonicalForm"/>
                <owl:onClass rdf:resource="&ontolex;Form"/>
                <owl:maxQualifiedCardinality rdf:datatype="&xsd;nonNegativeInteger">1</owl:maxQualifiedCardinality>
            </owl:Restriction>
        </rdfs:subClassOf>
        <rdfs:comment xml:lang="en">The class lexical entry represents a single unit of analysis in the lexicon comprising a collection of forms that are morphologically related or have a single pronunciation and have the same set of meanings.</rdfs:comment>
    </owl:Class>
    


    <!-- http://www.w3.org/ns/lemon/ontolex#LexicalSense -->

    <owl:Class rdf:about="&ontolex;LexicalSense">
        <rdfs:subClassOf rdf:resource="&semiotics;Meaning"/>
        <rdfs:subClassOf>
            <owl:Restriction>
                <owl:onProperty rdf:resource="&ontolex;reference"/>
                <owl:cardinality rdf:datatype="&xsd;nonNegativeInteger">1</owl:cardinality>
            </owl:Restriction>
        </rdfs:subClassOf>
        <rdfs:subClassOf>
            <owl:Restriction>
                <owl:onProperty rdf:resource="&ontolex;isSenseOf"/>
                <owl:onClass rdf:resource="&ontolex;LexicalEntry"/>
                <owl:qualifiedCardinality rdf:datatype="&xsd;nonNegativeInteger">1</owl:qualifiedCardinality>
            </owl:Restriction>
        </rdfs:subClassOf>
        <rdfs:comment xml:lang="en">The class lexical sense represents the lexical meaning of a lexical entry when interpreted as referring to the corresponding ontology element. A link between a lexical entry and an ontology entity via a LexicalSense object implies that the lexical entry can be used to refer to the ontology entity in question under corresponding connotations, pragmatic implications and meaning nuances that might no be directly modeled in the ontology. These pragmatic conditions and meaning nuances can be attached to the LexicalSense object, which represents a reification of the pair of LexicalEntry and ontology element. The Lexical Sense thus uniquely determines a lexical entry and an ontological entity it is associated with. </rdfs:comment>
    </owl:Class>
    


    <!-- http://www.w3.org/ns/lemon/ontolex#Lexicon -->

    <owl:Class rdf:about="&ontolex;Lexicon">
        <rdfs:subClassOf rdf:resource="http://rdfs.org/ns/void#Dataset"/>
        <rdfs:subClassOf>
            <owl:Restriction>
                <owl:onProperty rdf:resource="&ontolex;entry"/>
                <owl:onClass rdf:resource="&ontolex;LexicalEntry"/>
                <owl:minQualifiedCardinality rdf:datatype="&xsd;nonNegativeInteger">1</owl:minQualifiedCardinality>
            </owl:Restriction>
        </rdfs:subClassOf>
        <rdfs:comment xml:lang="en">The class lexicon represents a collection of lexical entries specific to the given language and/or domain. </rdfs:comment>
    </owl:Class>
    


    <!-- http://www.w3.org/ns/lemon/ontolex#MultiWordExpression -->

    <owl:Class rdf:about="&ontolex;MultiWordExpression">
        <rdfs:subClassOf rdf:resource="&ontolex;LexicalEntry"/>
        <rdfs:comment xml:lang="en">The class multiword expression represents a lexical entry consisting of two or more words. </rdfs:comment>
    </owl:Class>
    


    <!-- http://www.w3.org/ns/lemon/ontolex#Word -->

    <owl:Class rdf:about="&ontolex;Word">
        <rdfs:subClassOf rdf:resource="&ontolex;LexicalEntry"/>
        <rdfs:comment xml:lang="en">The class word represents a lexical entry consisting of a single word. </rdfs:comment>
    </owl:Class>
</rdf:RDF>



<!-- Generated by the OWL API (version 3.4.2) http://owlapi.sourceforge.net -->

