<?xml version="1.0"?>


<!DOCTYPE rdf:RDF [
    <!ENTITY owl "http://www.w3.org/2002/07/owl#" >
    <!ENTITY xsd "http://www.w3.org/2001/XMLSchema#" >
    <!ENTITY ontolex "http://www.w3.org/ns/lemon/ontolex#" >
    <!ENTITY rdfs "http://www.w3.org/2000/01/rdf-schema#" >
    <!ENTITY synsem "http://www.w3.org/ns/lemon/synsem.owl#" >
    <!ENTITY rdf "http://www.w3.org/1999/02/22-rdf-syntax-ns#" >
]>


<rdf:RDF xmlns="http://www.w3.org/ns/lemon/synsem.owl#"
     xml:base="http://www.w3.org/ns/lemon/synsem.owl"
     xmlns:rdfs="http://www.w3.org/2000/01/rdf-schema#"
     xmlns:synsem="http://www.w3.org/ns/lemon/synsem.owl#"
     xmlns:ontolex="http://www.w3.org/ns/lemon/ontolex#"
     xmlns:owl="http://www.w3.org/2002/07/owl#"
     xmlns:xsd="http://www.w3.org/2001/XMLSchema#"
     xmlns:rdf="http://www.w3.org/1999/02/22-rdf-syntax-ns#">
    <owl:Ontology rdf:about="http://www.w3.org/ns/lemon/synsem.owl">
        <owl:imports rdf:resource="http://www.w3.org/ns/lemon/ontolex"/>
    </owl:Ontology>
    


    <!-- 
    ///////////////////////////////////////////////////////////////////////////////////////
    //
    // Annotation properties
    //
    ///////////////////////////////////////////////////////////////////////////////////////
     -->

    


    <!-- http://www.w3.org/2000/01/rdf-schema#comment -->

    <owl:AnnotationProperty rdf:about="&rdfs;comment"/>
    


    <!-- 
    ///////////////////////////////////////////////////////////////////////////////////////
    //
    // Object Properties
    //
    ///////////////////////////////////////////////////////////////////////////////////////
     -->

    


    <!-- http://www.w3.org/2002/07/owl#topObjectProperty -->

    <owl:ObjectProperty rdf:about="&owl;topObjectProperty"/>
    


    <!-- http://www.w3.org/ns/lemon/synsem.owl#isA -->

    <owl:ObjectProperty rdf:about="&synsem;isA">
        <rdfs:comment xml:lang="en">The object property is a represents the single semantic argument of a class or unary  predicate.</rdfs:comment>
        <rdfs:subPropertyOf rdf:resource="&synsem;semArg"/>
    </owl:ObjectProperty>
    


    <!-- http://www.w3.org/ns/lemon/synsem.owl#marker -->

    <owl:ObjectProperty rdf:about="&synsem;marker">
        <rdfs:label xml:lang="en">marker</rdfs:label>
        <rdfs:comment xml:lang="en">The object property &apos;marker&apos; indicates the marker of a semantic argument; this can be a case marker or some other lexical entry such as a preposition or particle.</rdfs:comment>
        <rdfs:subPropertyOf rdf:resource="&owl;topObjectProperty"/>
        <rdfs:domain rdf:resource="&synsem;Argument"/>
    </owl:ObjectProperty>
    


    <!-- http://www.w3.org/ns/lemon/synsem.owl#objOfProp -->

    <owl:ObjectProperty rdf:about="&synsem;objOfProp">
        <rdfs:label xml:lang="en">object of property</rdfs:label>
        <rdfs:comment xml:lang="en">The object property &apos;object of property&apos; represents the semantic argument with represents the objects (range) of the property referred to by the semantic frame.</rdfs:comment>
        <rdfs:subPropertyOf rdf:resource="&owl;topObjectProperty"/>
        <rdfs:subPropertyOf rdf:resource="&synsem;semArg"/>
    </owl:ObjectProperty>
    


    <!-- http://www.w3.org/ns/lemon/synsem.owl#semArg -->

    <owl:ObjectProperty rdf:about="&synsem;semArg">
        <rdfs:label xml:lang="en">semantic argument</rdfs:label>
        <rdfs:comment xml:lang="en">The object property semantic argument represents an argument or slot of a semantic frame.</rdfs:comment>
        <rdfs:subPropertyOf rdf:resource="&owl;topObjectProperty"/>
        <rdfs:range rdf:resource="&synsem;Argument"/>
        <rdfs:domain rdf:resource="&synsem;SemanticFrame"/>
    </owl:ObjectProperty>
    


    <!-- http://www.w3.org/ns/lemon/synsem.owl#subjOfProp -->

    <owl:ObjectProperty rdf:about="&synsem;subjOfProp">
        <rdfs:label xml:lang="en">subject of property</rdfs:label>
        <rdfs:comment xml:lang="en">The object property &apos;subject of property&apos; represents the semantic argument with represents the subject (domain) of the property referred to by the semantic frame.</rdfs:comment>
        <rdfs:subPropertyOf rdf:resource="&owl;topObjectProperty"/>
        <rdfs:subPropertyOf rdf:resource="&synsem;semArg"/>
    </owl:ObjectProperty>
    


    <!-- http://www.w3.org/ns/lemon/synsem.owl#subsense -->

    <owl:ObjectProperty rdf:about="&synsem;subsense">
        <rdfs:label xml:lang="en">subsense</rdfs:label>
        <rdfs:comment xml:lang="en">Indicates that the relation between a compound sense and its atomic subsenses. It can be also used to relate a Semantic Frame to the single subframes that together compose the overall meaning as a Gestalt.
</rdfs:comment>
        <rdfs:subPropertyOf rdf:resource="&owl;topObjectProperty"/>
        <rdfs:domain rdf:resource="&ontolex;LexicalSense"/>
        <rdfs:range rdf:resource="&ontolex;LexicalSense"/>
    </owl:ObjectProperty>
    


    <!-- http://www.w3.org/ns/lemon/synsem.owl#synArg -->

    <owl:ObjectProperty rdf:about="&synsem;synArg">
        <rdfs:label xml:lang="en">syntactic argument</rdfs:label>
        <rdfs:comment xml:lang="en">The property syntactic argument relates a frame to one of its (syntactic) arguments. </rdfs:comment>
        <rdfs:subPropertyOf rdf:resource="&owl;topObjectProperty"/>
        <rdfs:range rdf:resource="&synsem;Argument"/>
        <rdfs:domain rdf:resource="&synsem;Frame"/>
    </owl:ObjectProperty>
    


    <!-- http://www.w3.org/ns/lemon/synsem.owl#synBehavior -->

    <owl:ObjectProperty rdf:about="&synsem;synBehavior">
        <rdfs:label xml:lang="en">syntactic behaviour</rdfs:label>
        <rdfs:comment xml:lang="en">The object property synBehavior relates a lexical entry to one of its syntactic behaviours as captured by a (syntactic) frame.</rdfs:comment>
        <rdfs:subPropertyOf rdf:resource="&owl;topObjectProperty"/>
        <rdfs:domain rdf:resource="&ontolex;LexicalEntry"/>
        <rdfs:range rdf:resource="&synsem;Frame"/>
    </owl:ObjectProperty>
    


    <!-- 
    ///////////////////////////////////////////////////////////////////////////////////////
    //
    // Data properties
    //
    ///////////////////////////////////////////////////////////////////////////////////////
     -->

    


    <!-- http://www.w3.org/2002/07/owl#topDataProperty -->

    <owl:DatatypeProperty rdf:about="&owl;topDataProperty">
        <rdfs:range rdf:resource="&xsd;boolean"/>
    </owl:DatatypeProperty>
    


    <!-- http://www.w3.org/ns/lemon/synsem.owl#optional -->

    <owl:DatatypeProperty rdf:about="&synsem;optional">
        <rdfs:comment xml:lang="en">Denotes that the syntactic argument is optional, that is, it may be omitted.
</rdfs:comment>
        <rdfs:range rdf:resource="&xsd;boolean"/>
        <rdfs:subPropertyOf rdf:resource="&owl;topDataProperty"/>
        <rdfs:domain rdf:resource="&synsem;Argument"/>
    </owl:DatatypeProperty>
    


    <!-- 
    ///////////////////////////////////////////////////////////////////////////////////////
    //
    // Classes
    //
    ///////////////////////////////////////////////////////////////////////////////////////
     -->

    


    <!-- http://www.w3.org/ns/lemon/ontolex#LexicalEntry -->

    <owl:Class rdf:about="&ontolex;LexicalEntry"/>
    


    <!-- http://www.w3.org/ns/lemon/ontolex#LexicalSense -->

    <owl:Class rdf:about="&ontolex;LexicalSense"/>
    


    <!-- http://www.w3.org/ns/lemon/synsem.owl#Argument -->

    <owl:Class rdf:about="&synsem;Argument">
        <rdfs:label xml:lang="en">Argument</rdfs:label>
        <rdfs:comment xml:lang="en">The class argument represents a slot that needs to be filled for a certain syntactic or semantic structure of a lexical entry or a semantic frame to be complete. Syntactic arguments typically realise a certain grammatical function (e.g. subject, direct object, indirect object, prepositional object, etc.); semantic arguments represent an entity that plays some role in a semantic frame.</rdfs:comment>
    </owl:Class>
    


    <!-- http://www.w3.org/ns/lemon/synsem.owl#Frame -->

    <owl:Class rdf:about="&synsem;Frame">
        <rdfs:label xml:lang="en">Frame</rdfs:label>
        <rdfs:comment xml:lang="en">The class (syntactic) frame represents the syntactic behaviour of an open class word in terms of (syntactic) arguments it requires. It essentially describes the subcategorization structure of the open class word in question, in particular the (syntactic) arguments it requires. </rdfs:comment>
    </owl:Class>
    


    <!-- http://www.w3.org/ns/lemon/synsem.owl#SemanticFrame -->

    <owl:Class rdf:about="&synsem;SemanticFrame">
        <rdfs:subClassOf rdf:resource="&ontolex;LexicalSense"/>
        <rdfs:comment xml:lang="en">The class semantic frame represents a coherent structure of related concepts that are related such that without knowledge of all of them, one does not have complete knowledge of any one; they are in that sense types of gestalt. The coherent structure is represented by one or more predicates from a given ontology.</rdfs:comment>
    </owl:Class>
</rdf:RDF>



<!-- Generated by the OWL API (version 3.4.2) http://owlapi.sourceforge.net -->

