<?xml version="1.0"?>


<!DOCTYPE rdf:RDF [
    <!ENTITY owl "http://www.w3.org/2002/07/owl#" >
    <!ENTITY xsd "http://www.w3.org/2001/XMLSchema#" >
    <!ENTITY ontolex "http://www.w3.org/ns/lemon/ontolex#" >
    <!ENTITY rdfs "http://www.w3.org/2000/01/rdf-schema#" >
    <!ENTITY synsem "http://www.w3.org/ns/lemon/synsem.owl#" >
    <!ENTITY rdf "http://www.w3.org/1999/02/22-rdf-syntax-ns#" >
]>


<rdf:RDF xmlns="http://www.w3.org/ns/lemon/synsem.owl#"
     xml:base="http://www.w3.org/ns/lemon/synsem.owl"
     xmlns:rdfs="http://www.w3.org/2000/01/rdf-schema#"
     xmlns:synsem="http://www.w3.org/ns/lemon/synsem.owl#"
     xmlns:ontolex="http://www.w3.org/ns/lemon/ontolex#"
     xmlns:owl="http://www.w3.org/2002/07/owl#"
     xmlns:xsd="http://www.w3.org/2001/XMLSchema#"
     xmlns:rdf="http://www.w3.org/1999/02/22-rdf-syntax-ns#">
    <owl:Ontology rdf:about="http://www.w3.org/ns/lemon/synsem.owl">
        <owl:imports rdf:resource="http://www.w3.org/ns/lemon/ontolex"/>
    </owl:Ontology>
    


    <!-- 
    ///////////////////////////////////////////////////////////////////////////////////////
    //
    // Annotation properties
    //
    ///////////////////////////////////////////////////////////////////////////////////////
     -->

    


    <!-- http://www.w3.org/2000/01/rdf-schema#comment -->

    <owl:AnnotationProperty rdf:about="&rdfs;comment"/>
    


    <!-- 
    ///////////////////////////////////////////////////////////////////////////////////////
    //
    // Object Properties
    //
    ///////////////////////////////////////////////////////////////////////////////////////
     -->

    


    <!-- http://www.w3.org/2002/07/owl#topObjectProperty -->

    <owl:ObjectProperty rdf:about="&owl;topObjectProperty"/>
    


    <!-- http://www.w3.org/ns/lemon/synsem.owl#condition -->

    <owl:ObjectProperty rdf:about="&synsem;condition">
        <rdfs:label xml:lang="en">condition</rdfs:label>
        <rdfs:comment xml:lang="en">The property condition defines an evaluable restriction on the mapping of this semantic frame.</rdfs:comment>
        <rdfs:subPropertyOf rdf:resource="&ontolex;usage"/>
        <rdfs:domain rdf:resource="&synsem;SemanticFrame"/>
    </owl:ObjectProperty>
    


    <!-- http://www.w3.org/ns/lemon/synsem.owl#isA -->

    <owl:ObjectProperty rdf:about="&synsem;isA">
        <rdfs:comment xml:lang="en">The object property is a represents the single semantic argument of a class or unary  predicate.</rdfs:comment>
        <rdfs:subPropertyOf rdf:resource="&synsem;semArg"/>
    </owl:ObjectProperty>
    


    <!-- http://www.w3.org/ns/lemon/synsem.owl#marker -->

    <owl:ObjectProperty rdf:about="&synsem;marker">
        <rdfs:label xml:lang="en">marker</rdfs:label>
        <rdfs:comment xml:lang="en">The object property marker indicates the marker of a semantic argument; this can be a case marker or some other lexical entry such as a preposition or particle.</rdfs:comment>
        <rdfs:subPropertyOf rdf:resource="&owl;topObjectProperty"/>
        <rdfs:domain rdf:resource="&synsem;SyntacticArgument"/>
    </owl:ObjectProperty>
    


    <!-- http://www.w3.org/ns/lemon/synsem.owl#objOfProp -->

    <owl:ObjectProperty rdf:about="&synsem;objOfProp">
        <rdfs:label xml:lang="en">object of property</rdfs:label>
        <rdfs:comment xml:lang="en">Indicates the semantic argument which represents the objects (range) of the property referred to by this semantic frame.</rdfs:comment>
        <rdfs:subPropertyOf rdf:resource="&owl;topObjectProperty"/>
        <rdfs:subPropertyOf rdf:resource="&synsem;semArg"/>
    </owl:ObjectProperty>
    


    <!-- http://www.w3.org/ns/lemon/synsem.owl#propertyDomain -->

    <owl:ObjectProperty rdf:about="&synsem;propertyDomain">
        <rdfs:label xml:lang="en">property domain</rdfs:label>
        <rdfs:comment xml:lang="en">&apos;Property domain&apos; provides a pragmatic restriction on the domain of the property referred to by this sense.</rdfs:comment>
        <rdfs:subPropertyOf rdf:resource="&synsem;condition"/>
    </owl:ObjectProperty>
    


    <!-- http://www.w3.org/ns/lemon/synsem.owl#propertyRange -->

    <owl:ObjectProperty rdf:about="&synsem;propertyRange">
        <rdfs:label xml:lang="en">property range</rdfs:label>
        <rdfs:comment xml:lang="en">&apos;Property domain&apos; provides a pragmatic restriction on the range of the property referred to by this sense.</rdfs:comment>
        <rdfs:subPropertyOf rdf:resource="&synsem;condition"/>
    </owl:ObjectProperty>
    


    <!-- http://www.w3.org/ns/lemon/synsem.owl#semArg -->

    <owl:ObjectProperty rdf:about="&synsem;semArg">
        <rdfs:label xml:lang="en">semantic argument</rdfs:label>
        <rdfs:comment xml:lang="en">The object property semArg represents an argument or slot of a semantic frame.</rdfs:comment>
        <rdfs:subPropertyOf rdf:resource="&owl;topObjectProperty"/>
        <rdfs:range rdf:resource="&synsem;SemanticArgument"/>
        <rdfs:domain rdf:resource="&synsem;SemanticFrame"/>
    </owl:ObjectProperty>
    


    <!-- http://www.w3.org/ns/lemon/synsem.owl#subframe -->

    <owl:ObjectProperty rdf:about="&synsem;subframe">
        <rdfs:label xml:lang="en">subframe</rdfs:label>
        <rdfs:comment xml:lang="en">The object property subframe relates a (complex) semantic frame to the subframes that together realize the maning of the whole subframe.</rdfs:comment>
        <rdfs:subPropertyOf rdf:resource="&owl;topObjectProperty"/>
        <rdfs:domain rdf:resource="&synsem;SemanticFrame"/>
        <rdfs:range rdf:resource="&synsem;SemanticFrame"/>
    </owl:ObjectProperty>
    


    <!-- http://www.w3.org/ns/lemon/synsem.owl#subjOfProp -->

    <owl:ObjectProperty rdf:about="&synsem;subjOfProp">
        <rdfs:label xml:lang="en">subject of property</rdfs:label>
        <rdfs:comment xml:lang="en">Indicates the semantic argument which represents the subjects (domain) of the property referred to by this sense.</rdfs:comment>
        <rdfs:subPropertyOf rdf:resource="&owl;topObjectProperty"/>
        <rdfs:subPropertyOf rdf:resource="&synsem;semArg"/>
    </owl:ObjectProperty>
    


    <!-- http://www.w3.org/ns/lemon/synsem.owl#synArg -->

    <owl:ObjectProperty rdf:about="&synsem;synArg">
        <rdfs:label xml:lang="en">syntactic argument</rdfs:label>
        <rdfs:comment xml:lang="en">The object property synArg relates a syntactic frame to one of its syntactic arguments.</rdfs:comment>
        <rdfs:subPropertyOf rdf:resource="&owl;topObjectProperty"/>
        <rdfs:range rdf:resource="&synsem;SyntacticArgument"/>
        <rdfs:domain rdf:resource="&synsem;SyntacticFrame"/>
    </owl:ObjectProperty>
    


    <!-- http://www.w3.org/ns/lemon/synsem.owl#synBehavior -->

    <owl:ObjectProperty rdf:about="&synsem;synBehavior">
        <rdfs:label xml:lang="en">syntactic behaviour</rdfs:label>
        <rdfs:comment xml:lang="en">The object property &apos;syntactic behaviour&apos; relates a lexical entry to one of its syntactic behaviours as captured by a syntactic frame.</rdfs:comment>
        <rdfs:subPropertyOf rdf:resource="&owl;topObjectProperty"/>
        <rdfs:domain rdf:resource="&ontolex;LexicalEntry"/>
        <rdfs:range rdf:resource="&synsem;SyntacticFrame"/>
    </owl:ObjectProperty>
    


    <!-- 
    ///////////////////////////////////////////////////////////////////////////////////////
    //
    // Data properties
    //
    ///////////////////////////////////////////////////////////////////////////////////////
     -->

    


    <!-- http://www.w3.org/2002/07/owl#topDataProperty -->

    <owl:DatatypeProperty rdf:about="&owl;topDataProperty">
        <rdfs:range rdf:resource="&xsd;boolean"/>
    </owl:DatatypeProperty>
    


    <!-- http://www.w3.org/ns/lemon/synsem.owl#optional -->

    <owl:DatatypeProperty rdf:about="&synsem;optional">
        <rdfs:label xml:lang="en">optional</rdfs:label>
        <rdfs:comment xml:lang="en">The datatype property &apos;optional&apos; indicates whether a syntactic argument is optional, that is, it can be syntactically ommitted.</rdfs:comment>
        <rdfs:range rdf:resource="&xsd;boolean"/>
        <rdfs:subPropertyOf rdf:resource="&owl;topDataProperty"/>
        <rdfs:domain rdf:resource="&synsem;SyntacticArgument"/>
    </owl:DatatypeProperty>
    


    <!-- 
    ///////////////////////////////////////////////////////////////////////////////////////
    //
    // Classes
    //
    ///////////////////////////////////////////////////////////////////////////////////////
     -->

    


    <!-- http://www.w3.org/ns/lemon/ontolex#LexicalEntry -->

    <owl:Class rdf:about="&ontolex;LexicalEntry"/>
    


    <!-- http://www.w3.org/ns/lemon/ontolex#LexicalSense -->

    <owl:Class rdf:about="&ontolex;LexicalSense"/>
    


    <!-- http://www.w3.org/ns/lemon/synsem.owl#Argument -->

    <owl:Class rdf:about="&synsem;Argument">
        <rdfs:label xml:lang="en">Argument</rdfs:label>
        <rdfs:comment xml:lang="en">The class argument represents a slot that needs to be filled for a certain syntactic or semantic structure of a lexical entry or a semantic frame to be complete. Syntactic arguments typically realise a certain grammatical function (e.g. subject, direct object, indirect object, prepositional object, etc.); semantic arguments represent an entity that plays some role in a semantic frame.</rdfs:comment>
    </owl:Class>
    


    <!-- http://www.w3.org/ns/lemon/synsem.owl#SemanticArgument -->

    <owl:Class rdf:about="&synsem;SemanticArgument">
        <rdfs:label xml:lang="en">Semantic Argument</rdfs:label>
        <rdfs:subClassOf rdf:resource="&synsem;Argument"/>
        <rdfs:comment xml:lang="en">The class SemanticArgument represents a slot that needs to be filled for a semantic frame to be complete. Semantic arguments typically express some actor or role played by some entity in the given semantic frame.</rdfs:comment>
    </owl:Class>
    


    <!-- http://www.w3.org/ns/lemon/synsem.owl#SemanticFrame -->

    <owl:Class rdf:about="&synsem;SemanticFrame">
        <rdfs:label xml:lang="en">Semantic Frame</rdfs:label>
        <owl:equivalentClass>
            <owl:Class>
                <owl:intersectionOf rdf:parseType="Collection">
                    <rdf:Description rdf:about="&ontolex;LexicalSense"/>
                    <owl:Restriction>
                        <owl:onProperty rdf:resource="&synsem;semArg"/>
                        <owl:someValuesFrom rdf:resource="&synsem;SemanticArgument"/>
                    </owl:Restriction>
                </owl:intersectionOf>
            </owl:Class>
        </owl:equivalentClass>
        <rdfs:subClassOf rdf:resource="&ontolex;LexicalSense"/>
        <rdfs:comment xml:lang="en">The class SemanticFrame captures the meaning of a lexical entry as expressed by one or more ontological predicates and their arguments. The different ontological predicates and their arguments form a whole and thus need all to be realized for the meaning to be complete.</rdfs:comment>
    </owl:Class>
    


    <!-- http://www.w3.org/ns/lemon/synsem.owl#SyntacticArgument -->

    <owl:Class rdf:about="&synsem;SyntacticArgument">
        <rdfs:label xml:lang="en">Syntactic Argument</rdfs:label>
        <rdfs:subClassOf rdf:resource="&synsem;Argument"/>
        <rdfs:comment xml:lang="en">The class syntactic argument represents a slot that needs to be filled for a certain syntactic or semantic structure of a lexical entry or a semantic frame to be complete. Syntactic arguments typically realise a certain grammatical function (e.g. subject, direct object, indirect object, prepositional object, etc.).</rdfs:comment>
    </owl:Class>
    


    <!-- http://www.w3.org/ns/lemon/synsem.owl#SyntacticFrame -->

    <owl:Class rdf:about="&synsem;SyntacticFrame">
        <rdfs:label xml:lang="en">Syntactic Frame</rdfs:label>
        <rdfs:comment xml:lang="en">The class syntactic frame represents the syntactic behaviour of an open class word in terms of (syntactic) arguments it requires. It essentially describes the subcategorization structure of the open class word in question, in particular the (syntactic) arguments it requires.</rdfs:comment>
    </owl:Class>
</rdf:RDF>



<!-- Generated by the OWL API (version 3.4.2) http://owlapi.sourceforge.net -->

