<?xml version="1.0"?>


<!DOCTYPE rdf:RDF [
    <!ENTITY owl "http://www.w3.org/2002/07/owl#" >
    <!ENTITY xsd "http://www.w3.org/2001/XMLSchema#" >
    <!ENTITY ontolex "http://www.w3.org/ns/lemon/ontolex#" >
    <!ENTITY rdfs "http://www.w3.org/2000/01/rdf-schema#" >
    <!ENTITY synsem "http://www.w3.org/ns/lemon/synsem.owl#" >
    <!ENTITY rdf "http://www.w3.org/1999/02/22-rdf-syntax-ns#" >
]>


<rdf:RDF xmlns="http://www.w3.org/ns/lemon/synsem.owl#"
     xml:base="http://www.w3.org/ns/lemon/synsem.owl"
     xmlns:rdfs="http://www.w3.org/2000/01/rdf-schema#"
     xmlns:synsem="http://www.w3.org/ns/lemon/synsem.owl#"
     xmlns:ontolex="http://www.w3.org/ns/lemon/ontolex#"
     xmlns:owl="http://www.w3.org/2002/07/owl#"
     xmlns:xsd="http://www.w3.org/2001/XMLSchema#"
     xmlns:rdf="http://www.w3.org/1999/02/22-rdf-syntax-ns#">
    <owl:Ontology rdf:about="http://www.w3.org/ns/lemon/synsem.owl">
        <owl:imports rdf:resource="http://www.w3.org/ns/lemon/ontolex"/>
    </owl:Ontology>
    


    <!-- 
    ///////////////////////////////////////////////////////////////////////////////////////
    //
    // Annotation properties
    //
    ///////////////////////////////////////////////////////////////////////////////////////
     -->

    


    <!-- http://www.w3.org/2000/01/rdf-schema#comment -->

    <owl:AnnotationProperty rdf:about="&rdfs;comment"/>
    


    <!-- 
    ///////////////////////////////////////////////////////////////////////////////////////
    //
    // Object Properties
    //
    ///////////////////////////////////////////////////////////////////////////////////////
     -->

    


    <!-- http://www.w3.org/2002/07/owl#topObjectProperty -->

    <owl:ObjectProperty rdf:about="&owl;topObjectProperty"/>
    


    <!-- http://www.w3.org/ns/lemon/synsem.owl#condition -->

    <owl:ObjectProperty rdf:about="&synsem;condition">
        <rdfs:comment xml:lang="en">Indicates a pragmatic restriction on the applicability of this sense</rdfs:comment>
        <rdfs:range rdf:resource="&ontolex;LexicalSense"/>
    </owl:ObjectProperty>
    


    <!-- http://www.w3.org/ns/lemon/synsem.owl#isA -->

    <owl:ObjectProperty rdf:about="&synsem;isA">
        <rdfs:comment xml:lang="en">Indicates the single semantic argument of a class or unary  predicate.</rdfs:comment>
        <rdfs:subPropertyOf rdf:resource="&synsem;semArg"/>
    </owl:ObjectProperty>
    


    <!-- http://www.w3.org/ns/lemon/synsem.owl#marker -->

    <owl:ObjectProperty rdf:about="&synsem;marker">
        <rdfs:comment xml:lang="en">Denotes the marker of a semantic argument. This should generally either be a semantic property i.e., case or another lexical entry e.g., a preposition or particle.</rdfs:comment>
        <rdfs:subPropertyOf rdf:resource="&owl;topObjectProperty"/>
        <rdfs:domain rdf:resource="&synsem;Argument"/>
    </owl:ObjectProperty>
    


    <!-- http://www.w3.org/ns/lemon/synsem.owl#objOfProp -->

    <owl:ObjectProperty rdf:about="&synsem;objOfProp">
        <rdfs:comment xml:lang="en">Indicates the semantic argument which represents the objects (range) of the property referred to by this sense.</rdfs:comment>
        <rdfs:subPropertyOf rdf:resource="&owl;topObjectProperty"/>
        <rdfs:subPropertyOf rdf:resource="&synsem;semArg"/>
    </owl:ObjectProperty>
    


    <!-- http://www.w3.org/ns/lemon/synsem.owl#propertyDomain -->

    <owl:ObjectProperty rdf:about="&synsem;propertyDomain">
        <rdfs:comment xml:lang="en">Provides a pragmatic restriction on the domain of the property referred to by this sense</rdfs:comment>
        <rdfs:domain rdf:resource="&ontolex;LexicalSense"/>
        <rdfs:subPropertyOf rdf:resource="&synsem;condition"/>
    </owl:ObjectProperty>
    


    <!-- http://www.w3.org/ns/lemon/synsem.owl#propertyRange -->

    <owl:ObjectProperty rdf:about="&synsem;propertyRange">
        <rdfs:comment xml:lang="en">Provides a pragmatic restriction on the range of the property referred to by this sense</rdfs:comment>
        <rdfs:domain rdf:resource="&ontolex;LexicalSense"/>
        <rdfs:subPropertyOf rdf:resource="&synsem;condition"/>
    </owl:ObjectProperty>
    


    <!-- http://www.w3.org/ns/lemon/synsem.owl#semArg -->

    <owl:ObjectProperty rdf:about="&synsem;semArg">
        <rdfs:comment xml:lang="en">Denotes a semantic argument slot of a semantic unit.</rdfs:comment>
        <rdfs:subPropertyOf rdf:resource="&owl;topObjectProperty"/>
        <rdfs:range rdf:resource="&synsem;Argument"/>
        <rdfs:domain rdf:resource="&synsem;SemanticFrame"/>
    </owl:ObjectProperty>
    


    <!-- http://www.w3.org/ns/lemon/synsem.owl#subjOfProp -->

    <owl:ObjectProperty rdf:about="&synsem;subjOfProp">
        <rdfs:comment xml:lang="en">Indicates the semantic argument which represents the subjects (domain) of the property referred to by this sense</rdfs:comment>
        <rdfs:subPropertyOf rdf:resource="&owl;topObjectProperty"/>
        <rdfs:subPropertyOf rdf:resource="&synsem;semArg"/>
    </owl:ObjectProperty>
    


    <!-- http://www.w3.org/ns/lemon/synsem.owl#subsense -->

    <owl:ObjectProperty rdf:about="&synsem;subsense">
        <rdfs:comment xml:lang="en">Indicates that the relation between a compound sense and its atomic subsenses. It can be also used to relate a Semantic Frame to the single subframes that together compose the overall meaning as a Gestalt.
</rdfs:comment>
        <rdfs:subPropertyOf rdf:resource="&owl;topObjectProperty"/>
        <rdfs:domain rdf:resource="&ontolex;LexicalSense"/>
        <rdfs:range rdf:resource="&ontolex;LexicalSense"/>
    </owl:ObjectProperty>
    


    <!-- http://www.w3.org/ns/lemon/synsem.owl#synArg -->

    <owl:ObjectProperty rdf:about="&synsem;synArg">
        <rdfs:comment xml:lang="en">The property synArg relates a Frame to one of its (syntactic) arguments.</rdfs:comment>
        <rdfs:subPropertyOf rdf:resource="&owl;topObjectProperty"/>
        <rdfs:range rdf:resource="&synsem;Argument"/>
        <rdfs:domain rdf:resource="&synsem;Frame"/>
    </owl:ObjectProperty>
    


    <!-- http://www.w3.org/ns/lemon/synsem.owl#synBehavior -->

    <owl:ObjectProperty rdf:about="&synsem;synBehavior">
        <rdfs:comment xml:lang="en">Indicates a syntactic behavior of a lexical entry</rdfs:comment>
        <rdfs:subPropertyOf rdf:resource="&owl;topObjectProperty"/>
        <rdfs:domain rdf:resource="&ontolex;LexicalEntry"/>
        <rdfs:range rdf:resource="&synsem;Frame"/>
    </owl:ObjectProperty>
    


    <!-- 
    ///////////////////////////////////////////////////////////////////////////////////////
    //
    // Data properties
    //
    ///////////////////////////////////////////////////////////////////////////////////////
     -->

    


    <!-- http://www.w3.org/2002/07/owl#topDataProperty -->

    <owl:DatatypeProperty rdf:about="&owl;topDataProperty">
        <rdfs:range rdf:resource="&xsd;boolean"/>
    </owl:DatatypeProperty>
    


    <!-- http://www.w3.org/ns/lemon/synsem.owl#optional -->

    <owl:DatatypeProperty rdf:about="&synsem;optional">
        <rdfs:comment xml:lang="en">Denotes that the syntactic argument is optional, that is, it may be omitted.
</rdfs:comment>
        <rdfs:range rdf:resource="&xsd;boolean"/>
        <rdfs:subPropertyOf rdf:resource="&owl;topDataProperty"/>
        <rdfs:domain rdf:resource="&synsem;Argument"/>
    </owl:DatatypeProperty>
    


    <!-- 
    ///////////////////////////////////////////////////////////////////////////////////////
    //
    // Classes
    //
    ///////////////////////////////////////////////////////////////////////////////////////
     -->

    


    <!-- http://www.w3.org/ns/lemon/ontolex#LexicalEntry -->

    <owl:Class rdf:about="&ontolex;LexicalEntry"/>
    


    <!-- http://www.w3.org/ns/lemon/ontolex#LexicalSense -->

    <owl:Class rdf:about="&ontolex;LexicalSense"/>
    


    <!-- http://www.w3.org/ns/lemon/synsem.owl#Argument -->

    <owl:Class rdf:about="&synsem;Argument">
        <rdfs:comment xml:lang="en">An argument represents a slot that needs to be filled for a certain syntactic structure/projection of a lexical entry or a semantic frame to be complete. Syntactic arguments typically realise a certain grammatical function (e.g. subject, direct object, indirect object, prepositional object, etc.); semantic arguments represent an entity that plays some role in a semantic frame.</rdfs:comment>
    </owl:Class>
    


    <!-- http://www.w3.org/ns/lemon/synsem.owl#Frame -->

    <owl:Class rdf:about="&synsem;Frame">
        <rdfs:comment xml:lang="en">A (syntactic) frame is a linguistic object that represents the syntactic behaviour of an open class word in terms of (syntactic) arguments it requires. It essentially describes the subcategorization structure of the open class word in question, in particular the (syntactic) arguments it requires.</rdfs:comment>
    </owl:Class>
    


    <!-- http://www.w3.org/ns/lemon/synsem.owl#SemanticFrame -->

    <owl:Class rdf:about="&synsem;SemanticFrame">
        <rdfs:subClassOf rdf:resource="&ontolex;LexicalSense"/>
        <rdfs:comment xml:lang="en">A semantic frame is a coherent structure of related concepts that are related such that without knowledge of all of them, one does not have complete knowledge of any one; they are in that sense types of gestalt. The coherent structure is represented by one or more predicates from a given ontology.</rdfs:comment>
    </owl:Class>
</rdf:RDF>



<!-- Generated by the OWL API (version 3.4.2) http://owlapi.sourceforge.net -->

