<?xml version="1.0"?>


<!DOCTYPE rdf:RDF [
    <!ENTITY owl "http://www.w3.org/2002/07/owl#" >
    <!ENTITY xsd "http://www.w3.org/2001/XMLSchema#" >
    <!ENTITY ontolex "http://www.w3.org/ns/lemon/ontolex#" >
    <!ENTITY rdfs "http://www.w3.org/2000/01/rdf-schema#" >
    <!ENTITY vartrans "http://www.w3.org/ns/lemon/vartrans.owl#" >
    <!ENTITY rdf "http://www.w3.org/1999/02/22-rdf-syntax-ns#" >
]>


<rdf:RDF xmlns="http://www.w3.org/ns/lemon/vartrans.owl#"
     xml:base="http://www.w3.org/ns/lemon/vartrans.owl"
     xmlns:vartrans="http://www.w3.org/ns/lemon/vartrans.owl#"
     xmlns:rdfs="http://www.w3.org/2000/01/rdf-schema#"
     xmlns:ontolex="http://www.w3.org/ns/lemon/ontolex#"
     xmlns:owl="http://www.w3.org/2002/07/owl#"
     xmlns:xsd="http://www.w3.org/2001/XMLSchema#"
     xmlns:rdf="http://www.w3.org/1999/02/22-rdf-syntax-ns#">
    <owl:Ontology rdf:about="http://www.w3.org/ns/lemon/vartrans.owl">
        <owl:imports rdf:resource="http://www.w3.org/ns/lemon/ontolex"/>
    </owl:Ontology>
    


    <!-- 
    ///////////////////////////////////////////////////////////////////////////////////////
    //
    // Object Properties
    //
    ///////////////////////////////////////////////////////////////////////////////////////
     -->

    


    <!-- http://www.w3.org/2002/07/owl#topObjectProperty -->

    <owl:ObjectProperty rdf:about="&owl;topObjectProperty"/>
    


    <!-- http://www.w3.org/ns/lemon/vartrans.owl#category -->

    <owl:ObjectProperty rdf:about="&vartrans;category">
        <rdf:type rdf:resource="&owl;FunctionalProperty"/>
        <rdfs:label xml:lang="en">category</rdfs:label>
        <rdfs:comment xml:lang="en">The object property category indicates the specific type of relation by which two lexical entries or two lexical senses are related.</rdfs:comment>
        <rdfs:subPropertyOf rdf:resource="&owl;topObjectProperty"/>
        <rdfs:domain rdf:resource="&vartrans;LexicoSemanticRelation"/>
    </owl:ObjectProperty>
    


    <!-- http://www.w3.org/ns/lemon/vartrans.owl#context -->

    <owl:ObjectProperty rdf:about="&vartrans;context">
        <rdfs:label xml:lang="en">context</rdfs:label>
        <rdfs:comment xml:lang="en">The object property context indicates the contextual conditions under which a certain sense relation holds.</rdfs:comment>
        <rdfs:subPropertyOf rdf:resource="&owl;topObjectProperty"/>
        <rdfs:domain>
            <owl:Class>
                <owl:unionOf rdf:parseType="Collection">
                    <rdf:Description rdf:about="&ontolex;LexicalSense"/>
                    <rdf:Description rdf:about="&vartrans;LexicoSemanticRelation"/>
                </owl:unionOf>
            </owl:Class>
        </rdfs:domain>
    </owl:ObjectProperty>
    


    <!-- http://www.w3.org/ns/lemon/vartrans.owl#lexicalRel -->

    <owl:ObjectProperty rdf:about="&vartrans;lexicalRel">
        <rdfs:label xml:lang="en">lexical relation</rdfs:label>
        <rdfs:comment xml:lang="en">The object property lexicalRel relates two lexical entries that stand in some lexical relation.</rdfs:comment>
        <rdfs:domain rdf:resource="&ontolex;LexicalEntry"/>
        <rdfs:range rdf:resource="&ontolex;LexicalEntry"/>
    </owl:ObjectProperty>
    


    <!-- http://www.w3.org/ns/lemon/vartrans.owl#relates -->

    <owl:ObjectProperty rdf:about="&vartrans;relates">
        <rdfs:label xml:lang="en">relates</rdfs:label>
        <rdfs:comment xml:lang="en">The object property &apos;&apos;&apos;relates&apos;&apos;&apos; links a lexico-semantic relation to the two lexical entries or lexical senses between which it establishes the relation.</rdfs:comment>
        <rdfs:domain rdf:resource="&vartrans;LexicoSemanticRelation"/>
        <rdfs:range>
            <owl:Class>
                <owl:unionOf rdf:parseType="Collection">
                    <rdf:Description rdf:about="&ontolex;LexicalEntry"/>
                    <rdf:Description rdf:about="&ontolex;LexicalSense"/>
                </owl:unionOf>
            </owl:Class>
        </rdfs:range>
    </owl:ObjectProperty>
    


    <!-- http://www.w3.org/ns/lemon/vartrans.owl#senseRel -->

    <owl:ObjectProperty rdf:about="&vartrans;senseRel">
        <rdfs:label xml:lang="en">sense relation</rdfs:label>
        <rdfs:comment xml:lang="en">The object property senseRel relates to lexical senses that stand in some sense relation.</rdfs:comment>
        <rdfs:domain rdf:resource="&ontolex;LexicalSense"/>
        <rdfs:range rdf:resource="&ontolex;LexicalSense"/>
    </owl:ObjectProperty>
    


    <!-- http://www.w3.org/ns/lemon/vartrans.owl#source -->

    <owl:ObjectProperty rdf:about="&vartrans;source">
        <rdf:type rdf:resource="&owl;FunctionalProperty"/>
        <rdfs:label xml:lang="en">source</rdfs:label>
        <rdfs:comment xml:lang="en">Source of a Variation.</rdfs:comment>
        <rdfs:domain rdf:resource="&vartrans;LexicoSemanticRelation"/>
        <rdfs:subPropertyOf rdf:resource="&vartrans;relates"/>
    </owl:ObjectProperty>
    


    <!-- http://www.w3.org/ns/lemon/vartrans.owl#target -->

    <owl:ObjectProperty rdf:about="&vartrans;target">
        <rdf:type rdf:resource="&owl;FunctionalProperty"/>
        <rdfs:label xml:lang="en">target</rdfs:label>
        <rdfs:comment xml:lang="en">Target of a Variation.</rdfs:comment>
        <rdfs:domain rdf:resource="&vartrans;LexicoSemanticRelation"/>
        <rdfs:subPropertyOf rdf:resource="&vartrans;relates"/>
    </owl:ObjectProperty>
    


    <!-- http://www.w3.org/ns/lemon/vartrans.owl#translatableAs -->

    <owl:ObjectProperty rdf:about="&vartrans;translatableAs">
        <rdf:type rdf:resource="&owl;SymmetricProperty"/>
        <rdfs:label xml:lang="en">translatableAs</rdfs:label>
        <rdfs:comment xml:lang="en">The object property translatableAs relates a lexical entry to a lexical entry that it can be translated as depending on the particular context and specific senses of the involved lexical entries.</rdfs:comment>
        <rdfs:range rdf:resource="&ontolex;LexicalEntry"/>
        <rdfs:domain rdf:resource="&ontolex;LexicalEntry"/>
        <rdfs:subPropertyOf rdf:resource="&vartrans;lexicalRel"/>
    </owl:ObjectProperty>
    


    <!-- 
    ///////////////////////////////////////////////////////////////////////////////////////
    //
    // Classes
    //
    ///////////////////////////////////////////////////////////////////////////////////////
     -->

    


    <!-- http://www.w3.org/ns/lemon/ontolex#Form -->

    <owl:Class rdf:about="&ontolex;Form"/>
    


    <!-- http://www.w3.org/ns/lemon/ontolex#LexicalEntry -->

    <owl:Class rdf:about="&ontolex;LexicalEntry"/>
    


    <!-- http://www.w3.org/ns/lemon/ontolex#LexicalSense -->

    <owl:Class rdf:about="&ontolex;LexicalSense"/>
    


    <!-- http://www.w3.org/ns/lemon/vartrans.owl#LexicalRelation -->

    <owl:Class rdf:about="&vartrans;LexicalRelation">
        <rdfs:label xml:lang="en">Lexical Relation</rdfs:label>
        <rdfs:subClassOf rdf:resource="&vartrans;LexicoSemanticRelation"/>
        <rdfs:subClassOf>
            <owl:Restriction>
                <owl:onProperty rdf:resource="&vartrans;relates"/>
                <owl:onClass rdf:resource="&ontolex;LexicalEntry"/>
                <owl:qualifiedCardinality rdf:datatype="&xsd;nonNegativeInteger">2</owl:qualifiedCardinality>
            </owl:Restriction>
        </rdfs:subClassOf>
        <rdfs:comment xml:lang="en">The class &apos;&apos;&apos;lexical relation&apos;&apos;&apos; reifies the relation between two lexical entries that are related by some lexical relation.</rdfs:comment>
    </owl:Class>
    


    <!-- http://www.w3.org/ns/lemon/vartrans.owl#LexicoSemanticRelation -->

    <owl:Class rdf:about="&vartrans;LexicoSemanticRelation">
        <rdfs:label xml:lang="en">Lexico-Semantic Relation</rdfs:label>
        <rdfs:subClassOf>
            <owl:Restriction>
                <owl:onProperty rdf:resource="&vartrans;relates"/>
                <owl:onClass>
                    <owl:Class>
                        <owl:unionOf rdf:parseType="Collection">
                            <rdf:Description rdf:about="&ontolex;Form"/>
                            <rdf:Description rdf:about="&ontolex;LexicalEntry"/>
                            <rdf:Description rdf:about="&ontolex;LexicalSense"/>
                        </owl:unionOf>
                    </owl:Class>
                </owl:onClass>
                <owl:qualifiedCardinality rdf:datatype="&xsd;nonNegativeInteger">2</owl:qualifiedCardinality>
            </owl:Restriction>
        </rdfs:subClassOf>
        <rdfs:comment xml:lang="en">The class lexico-semantic relation reifies the relation between two lexical entries or lexical senses that are related by some lexical or semantic relationship.</rdfs:comment>
    </owl:Class>
    


    <!-- http://www.w3.org/ns/lemon/vartrans.owl#SenseRelation -->

    <owl:Class rdf:about="&vartrans;SenseRelation">
        <rdfs:label xml:lang="en">Sense Relation</rdfs:label>
        <rdfs:subClassOf rdf:resource="&vartrans;LexicoSemanticRelation"/>
        <rdfs:subClassOf>
            <owl:Restriction>
                <owl:onProperty rdf:resource="&vartrans;relates"/>
                <owl:onClass rdf:resource="&ontolex;LexicalSense"/>
                <owl:qualifiedCardinality rdf:datatype="&xsd;nonNegativeInteger">2</owl:qualifiedCardinality>
            </owl:Restriction>
        </rdfs:subClassOf>
        <rdfs:comment xml:lang="en">The class sense relation reifies the relation between two lexical entries that are related by a relation.</rdfs:comment>
    </owl:Class>
    


    <!-- http://www.w3.org/ns/lemon/vartrans.owl#TerminologicalRelation -->

    <owl:Class rdf:about="&vartrans;TerminologicalRelation">
        <rdfs:label xml:lang="en">Terminological Relation</rdfs:label>
        <rdfs:subClassOf rdf:resource="&vartrans;SenseRelation"/>
        <rdfs:comment xml:lang="en">The class terminological relation reifies the relation between terms that are semantically related in the sense that they can be exchanged in most contexts, but their surface forms are not directly related. The variants vary along dimensions that are not captured by the given ontology and are intentionally (pragmatically) caused.</rdfs:comment>
    </owl:Class>
    


    <!-- http://www.w3.org/ns/lemon/vartrans.owl#Translation -->

    <owl:Class rdf:about="&vartrans;Translation">
        <rdfs:label xml:lang="en">Translation</rdfs:label>
        <rdfs:subClassOf rdf:resource="&vartrans;SenseRelation"/>
        <rdfs:subClassOf>
            <owl:Restriction>
                <owl:onProperty rdf:resource="&vartrans;target"/>
                <owl:onClass rdf:resource="&ontolex;LexicalSense"/>
                <owl:qualifiedCardinality rdf:datatype="&xsd;nonNegativeInteger">1</owl:qualifiedCardinality>
            </owl:Restriction>
        </rdfs:subClassOf>
        <rdfs:comment xml:lang="en">The class translation represents a special case of SenseRelation involving two lexical senses that correspond to two lexical entries in different languages that stand in a translation relation so that they can be exchanged without any meaning implications.</rdfs:comment>
    </owl:Class>
</rdf:RDF>



<!-- Generated by the OWL API (version 3.4.2) http://owlapi.sourceforge.net -->

